Fix

SmullyanSystem/Basic.lean
@@ -8,181 +8,141 @@ structure SmullyanModel where
   α : Type*
   isPredicate : List α → Prop
   isPredicate_spec : ∀ p : { x // isPredicate x }, ∀ x ≠ [], ¬isPredicate (p.val ++ x)
-  val : { x // isPredicate x } → Set (List α)
+  valuation : { x // isPredicate x } → Set (List α)
 
 namespace SmullyanModel
 
-section
-
-variable (M : SmullyanModel)
-
-abbrev Word := List M.α
-
-abbrev words : Set M.Word := Set.univ
-
-abbrev epsilon : M.Word := []
+variable {M : SmullyanModel}
 
 
-abbrev Predicate := { P // M.isPredicate P }
+abbrev Word (M : SmullyanModel) := List M.α
 
-abbrev predicates : Set M.Predicate := Set.univ
+abbrev words (M : SmullyanModel) : Set M.Word := Set.univ
+
+abbrev epsilon (M : SmullyanModel) : M.Word := []
+
+
+abbrev Predicate (M : SmullyanModel) := { P // M.isPredicate P }
+
+abbrev predicates (M : SmullyanModel) : Set M.Predicate := Set.univ
 
 instance : Coe (Set M.Predicate) (Set M.Word) := ⟨fun s => s.image (·.val)⟩
 
 @[simp] lemma isPredicate_predicate {P : M.Predicate} : M.isPredicate P.val := P.property
 
+def Predicate.valuated (P : M.Predicate) : Set M.Word := M.valuation P
 
-structure Sentence where
+def Predicate.names (P : M.Predicate) (V : Set M.Word) : Prop := P.valuated = V
+
+
+structure Sentence (M : SmullyanModel) where
   P : M.Predicate
   W : M.Word
 
-abbrev sentences : Set M.Sentence := Set.univ
+abbrev sentences (M : SmullyanModel) : Set M.Sentence := Set.univ
 
-abbrev Sentence.toWord {M : SmullyanModel} : M.Sentence → M.Word := fun ⟨P, W⟩ => P ++ W
+def Sentence.toWord : M.Sentence → M.Word := fun ⟨P, W⟩ => P ++ W
 
 instance : Coe (M.Sentence) (M.Word) := ⟨Sentence.toWord⟩
 
 instance : Coe (Set M.Sentence) (Set M.Word) := ⟨fun s => s.image Sentence.toWord⟩
 
-@[simp] lemma Sentence.iff_toWord {M : SmullyanModel} {S : M.Sentence} : S.toWord = S.P ++ S.W := by rfl
+@[simp] lemma Sentence.iff_toWord {S : M.Sentence} : S.toWord = S.P ++ S.W := by rfl
 
 def isSentence (W : M.Word) : Prop := ∃ S : M.Sentence, W = S
 
 @[simp] lemma isSentence_sentence {S : M.Sentence} : M.isSentence S := ⟨S, rfl⟩
 
 
-structure ProperSentence extends M.Sentence where
+
+structure ProperSentence (M : SmullyanModel) extends M.Sentence where
   W_nonempty : W ≠ []
-abbrev proper_sentences : Set M.ProperSentence := Set.univ
+
+abbrev proper_sentences (M : SmullyanModel) : Set M.ProperSentence := Set.univ
+
 def isProperSentence (W : M.Word) : Prop := M.isSentence W ∧ ¬M.isPredicate W
 
 
-def Predicate.names {M : SmullyanModel} (P : M.Predicate) (V : Set M.Word) := M.val P = V
+def true_sentences (M : SmullyanModel) : Set M.Sentence := fun ⟨P, W⟩ => W ∈ P.valuated
+
+def true_proper_sentences (M : SmullyanModel) : Set M.ProperSentence := fun ⟨⟨P, W⟩, _⟩ => W ∈ M.valuation P
+
+def false_sentences (M : SmullyanModel) : Set M.Sentence := M.sentences \ M.true_sentences
+
+def false_proper_sentences (M : SmullyanModel) : Set M.ProperSentence := M.proper_sentences \ M.true_proper_sentences
 
 
-def true_sentences : Set M.Sentence := fun ⟨P, W⟩ => W ∈ M.val P
-
-def true_proper_sentences : Set M.ProperSentence := fun ⟨⟨P, W⟩, _⟩ => W ∈ M.val P
-
-def false_sentences : Set M.Sentence := M.sentences \ M.true_sentences
-
-def false_proper_sentences : Set M.ProperSentence := M.proper_sentences \ M.true_proper_sentences
-
-
-
-
-def Sentence.isTrue {M : SmullyanModel} (S : M.Sentence) := S ∈ M.true_sentences
+def Sentence.isTrue (S : M.Sentence) := S ∈ M.true_sentences
 prefix:90 "⊨ " => Sentence.isTrue
 
-class IsN where
+@[simp] lemma iff_mem_true_sentences : ⊨ S ↔ S.W ∈ S.P.valuated := by rfl
+
+
+
+class IsN (M : SmullyanModel) where
   n : M.α
   n_spec₁ : ∀ P : M.Predicate, (M.isPredicate (n :: P))
-  n_spec₂ : ∀ P : M.Predicate, M.val ⟨n :: P, n_spec₁ P⟩ = M.words \ M.val P
+  n_spec₂ : ∀ P : M.Predicate, M.valuation ⟨n :: P, n_spec₁ P⟩ = (P.valuated)ᶜ
 
 section
 
-variable {M} [M.IsN]
+variable [M.IsN]
 
-abbrev Predicate.negated (P : M.Predicate) : M.Predicate := ⟨IsN.n :: P.val, IsN.n_spec₁ P⟩
+def Predicate.negated (P : M.Predicate) : M.Predicate := ⟨IsN.n :: P.val, IsN.n_spec₁ P⟩
 prefix:90 "~" => Predicate.negated
 
-abbrev Sentence.negated (S : M.Sentence) : M.Sentence := ⟨⟨IsN.n :: S.P, IsN.n_spec₁ S.P⟩, S.W⟩
+def Sentence.negated (S : M.Sentence) : M.Sentence := ⟨~S.P, S.W⟩
 prefix:90 "~" => Sentence.negated
 
 def Sentence.isNegTrue (S : M.Sentence) := ⊨ ~S
 prefix:50 "⊭ " => Sentence.isNegTrue
 
-@[simp] lemma IsN.n_spec₂' {P : M.Predicate} : M.val (~P) = (M.val P)ᶜ := by simp [IsN.n_spec₂ P]; aesop;
+@[simp]
+lemma iff_negated_valuated {P : M.Predicate} : (~P).valuated = P.valuatedᶜ := by
+  simp [Predicate.valuated, Predicate.negated, IsN.n_spec₂ P];
 
 end
 
 
-class IsR where
+class IsR (M : SmullyanModel) where
   r : M.α
   r_spec₁ : ∀ P : M.Predicate, (M.isPredicate (r :: P))
-  r_spec₂ : ∀ P : M.Predicate, M.val ⟨r :: P, r_spec₁ P⟩ = { K : M.Predicate | K.val ++ K.val ∈ M.val P }
+  r_spec₂ : ∀ P : M.Predicate, M.valuation ⟨r :: P, r_spec₁ P⟩ = { K : M.Predicate | K.val ++ K.val ∈ P.valuated }
 
 section
 
-variable {M} [M.IsR]
+variable [M.IsR]
 
-abbrev Predicate.repeated (P : M.Predicate) : M.Predicate := ⟨IsR.r :: P.val, IsR.r_spec₁ P⟩
+def Predicate.repeated (P : M.Predicate) : M.Predicate := ⟨IsR.r :: P.val, IsR.r_spec₁ P⟩
 prefix:90 "□" => Predicate.repeated
 
-abbrev Sentence.repeated (S : M.Sentence) : M.Sentence := ⟨⟨IsR.r :: S.P.val, IsR.r_spec₁ S.P⟩, S.W⟩
+def Sentence.repeated (S : M.Sentence) : M.Sentence := ⟨□S.P, S.W⟩
 prefix:90 "□" => Sentence.repeated
 
-@[simp] lemma Predicate.repeated_isPredicate {P : M.Predicate} : M.isPredicate (□P) := IsR.r_spec₁ P
-@[simp] lemma Sentence.repeated_isSentence {S : M.Sentence} : M.isSentence (□S) := by use ⟨□S.P, S.W⟩;
-
-@[simp] lemma IsR.repeated_val {P : M.Predicate} : M.val (□P) = { K : M.Predicate | K.val ++ K.val ∈ M.val P } := by rw [IsR.r_spec₂ P];
-
-end
-
-
-class IsNR extends IsN M, IsR M where
+@[simp]
+lemma iff_repeated_valuated {P : M.Predicate} : (□P).valuated = { K : M.Predicate | K.val ++ K.val ∈ P.valuated } := by
+  simp [Predicate.valuated, Predicate.repeated, IsR.r_spec₂ P];
 
 end
 
 
+class IsNR (M : SmullyanModel) extends IsN M, IsR M where
 
-variable {M : SmullyanModel}
 
-@[simp] lemma iff_mem_true_sentences : ⊨ S ↔ S.W ∈ M.val S.P := by rfl
-
+variable {P : M.Predicate} {S : M.Sentence}
 
 def Predicate.fixpoint [M.IsR] (P : M.Predicate) : M.Sentence := ⟨□P, □P⟩
 
-theorem fixpoint_spec [M.IsR] {P : M.Predicate} : ⊨ P.fixpoint ↔ ⊨ (⟨P, P.fixpoint⟩) := by
-  simp_all [Predicate.fixpoint, Predicate.repeated_isPredicate];
-  intros;
-  exact Predicate.repeated_isPredicate;
+lemma fixpoint_spec [M.IsR] : ⊨ P.fixpoint ↔ ⊨ (⟨P, P.fixpoint⟩) := by simp [Predicate.fixpoint];
 
-/-
-lemma fixpoint_mem [M.IsNR] {P : M.Predicate} : ⊨ (~P).fixpoint ↔ ↑(~P).fixpoint ∉ M.val P := by
-  simp [Predicate.fixpoint];
-  intro;
-  exact Predicate.repeated_isPredicate;
-  constructor;
-  . intro h;
-    have := fixpoint_spec.mp h;
-    simp at this;
-    simp [fixpoint_spec]
-    simp only [iff_mem_true_sentences] at h;
-    simp only [iff_mem_true_sentences, Sentence.iff_toWord, Predicate.fixpoint];
-    intro h;
-    sorry;
-  . sorry;
+lemma iff_fixpoint_is_true [M.IsNR] : ⊨ (~P).fixpoint ↔ ↑(~P).fixpoint ∉ P.valuated := by simp [Predicate.fixpoint];
 
 theorem tarski [M.IsNR] : ¬∃ P : M.Predicate, P.names M.true_sentences := by
   by_contra hC;
-  obtain ⟨P, hP⟩ := hC;
-  simp [Predicate.names] at hP;
-  have := subset_of_eq hP;
+  sorry;
 
-  intro P;
-  simp only [Predicate.names];
-  suffices M.Φ P ⊂ M.true_sentences by exact ne_of_ssubset this;
-  by_cases hF : P.fixpoint ∈ M.true_sentences;
-  . constructor;
-    . sorry;
-    . sorry;
-  . constructor;
-    . sorry;
-    . sorry;
-  -- by_cases
-  constructor;
-  . intro W hW;
-    simp;
-    use ⟨P, W⟩;
-    constructor;
-    . sorry;
-    . sorry;
-  . apply Set.not_subset.mpr;
-    use P.fixpoint;
-    simp [fixpoint_spec];
-    sorry;
-  -- let F := P.fixpoint;
--/
+theorem goedel1 [M.IsNR] (hP : P.valuated ⊆ M.true_sentences) : ∃ S : M.Sentence, ↑S ∉ P.valuated ∧ ↑(~S) ∈ P.valuated := by
+  by_contra hC;
+  sorry;
 
 end SmullyanModel
